1) **If $A$ is nonsingular, and $AB=0$ then $B=0$.**
###### Why:
Since $A$ is non singular $A^{-1}$ exists. 
Since$$
AB=0
$$$$
A^{-1}(AB)=A^{-1}0
$$
$$
(A^{-1}A)B=0
$$
$$
B=0
$$
2) **If $A$ is nonsingular and $AB=AC$, then $B=C$**
###### Why:
$$
AB=AC
$$
$$
A^{-1}(AB)=A^{-1}(AC)
$$
$$
(A^{-1}A)B=(A^{-1}A)C
$$
$$
B=C
$$
#### Algebraic Properties:
3) **If $A$ is nonsingular and $\alpha \neq 0$, a scalar, then $\alpha \cdot A$ is also nonsingular** and $$
(\alpha \cdot A)^{-1}=\frac{1}{\alpha}  \cdot A^{-1}
$$
###### Why:
$$
(\alpha \cdot A)\cdot\left(  \frac{1}{\alpha} \cdot A^{-1} \right)
$$
$$
=I
$$
4) **If $A,B$ are nonsingular then $AB$ (and $BA$) is nonsingular and $(AB)^{-1}=$ $B^{-1}A^{-1}$**
###### Why:
$$
(AB)(B^{-1}A^{-1})
$$
$$
= A(BB^{-1})A^{-1}
$$
$$
= AIA^{-1}
$$
$$
=I
$$

5) **If $A,B$ are nonsingular, then $A+B$ may be nonsingular or singular, and if $A+B$ is nonsingular,**
$$
(A+B)^{-1} \neq A^{-1}+B^{-1}
$$

##### Property:
If
$$
A=\begin{bmatrix}
a & b \\
c & d
\end{bmatrix}
$$
and $ad-bc\neq 0$, then $A$ is nonsingular and
$$
A^{-1}=\frac{1}{ad-bc}\cdot \begin{bmatrix}
d & -b \\
-c & a
\end{bmatrix}
$$
5) If $A$ is non singular and p is any integer $\geq$ 1, $$
(A^P)^{-1} = (A^{-1})^P
$$